Cleanup and documentation

theories/eris/lib/sampling/bernoulli/implementation.v
@@ -1,3 +1,7 @@
+(**
+  This file implements the bernoulli distribution by giving a function that mimics it, and full specifications with our without tapes.
+*)
+
 From clutch.eris Require Import eris.
 From clutch.eris.lib.sampling.bernoulli Require Import tape lemmas interface.
 From clutch.eris.lib.sampling Require Import utils.
@@ -16,12 +20,18 @@ From clutch.eris.lib.sampling Require Import utils.
 
 Section BernoulliImpl.
   Context `{!erisGS Σ}.
-  
+
+  (**
+    The bernoulli distribution is a distribution on {0, 1} that succeeds with probability p (here `N / (M + 1)`) and fails with probability `1 - p`
+  *)
   Definition bernoulli : val := 
     λ: "α" "N" "M",
       let: "x" := rand("α") "M" in 
       if: "x" < "N" then #1 else #0.
 
+  (**
+    The base specification for tapeless usage, every other one can be derived from it
+  *)
   Lemma twp_bernoulli_scale (N M : nat) (ε ε1 ε2 : R) (p := N / S M) :
     (N ≤ S M)%nat →
     0 <= ε1 →
@@ -30,9 +40,9 @@ Section BernoulliImpl.
     [[{↯ ε}]]
       bernoulli #() #N #M
     [[{
-        (k : nat), RET #k; 
-        (⌜k = 0%nat⌝ ∗ ↯ ε1) ∨
-        (⌜k = 1%nat⌝ ∗ ↯ ε2)
+      (k : nat), RET #k; 
+      (⌜k = 0%nat⌝ ∗ ↯ ε1) ∨
+      (⌜k = 1%nat⌝ ∗ ↯ ε2)
     }]].
   Proof.
     iIntros (HNleM ε1_pos ε2_pos Heq Φ) "Herr HΦ".
@@ -46,10 +56,9 @@ Section BernoulliImpl.
       λ (n : fin (S M)), 
         if bool_decide (fin_to_nat n < N)%nat then ε2' else ε1' 
     .
-    wp_apply (twp_couple_rand_adv_comp1 _ _ _ ε' f with "Herr") as "%x Herr"; unfold f.
-    { move=>>;
-      by case_bool_decide. }
-    { rewrite SeriesC_scal_l. rewrite Rmult_comm.
+    wp_apply (twp_couple_rand_adv_comp1 _ _ _ ε' f with "Herr") as "%x Herr"; subst f.
+    { move=>> /=; by case_bool_decide. }
+    { rewrite SeriesC_scal_l Rmult_comm.
       simpl_expr.
       Opaque INR.
       setoid_rewrite ssrbool.fun_if.
@@ -61,11 +70,15 @@ Section BernoulliImpl.
       rewrite -(Rmult_assoc (S M) ε1 _) -(Rmult_comm ε1 (S M)) (Rmult_assoc ε1 (S M) _).
       simpl_expr. }
     wp_pures.
-    repeat case_bool_decide; wp_pures; try lia.
-    - iApply ("HΦ" $! 1)%nat; auto.
-    - iApply ("HΦ" $! 0)%nat; auto.
+    repeat case_bool_decide; try lia; wp_pures.
+    - iApply ("HΦ" $! 1)%nat; done.
+    - iApply ("HΦ" $! 0)%nat; done.
   Qed.
-  
+
+  (**
+    This is a lemma to do a case disjunction, it cannot be derived from `twp_bernoulli_scale` because it doesn't require 
+    `N ≤ M + 1`, but isn't very useful as it can't scale credits
+  *)
   Lemma bernoulli_case (N M : nat) :
     [[{True}]] 
       bernoulli #() #N #M 
@@ -78,8 +91,12 @@ Section BernoulliImpl.
     wp_pures; iApply "HΦ"; auto.
   Qed.
 
-  Definition own_bernoulli_tape α N M v := (∃ l, α ↪ (M; l) ∗ ⌜is_bernoulli_translation N M v l⌝)%I.
 
+  Definition own_bernoulli_tape α N M v : iProp Σ := ∃ l, α ↪ (M; l) ∗ ⌜is_bernoulli_translation N M v l⌝.
+
+  (**
+    Adaptation of the presample lemma for bernoulli distribution
+  *)
   Lemma twp_presample_bernoulli 
       (e : expr) (α : loc) (Φ : val → iProp Σ)
       (N M : nat) (ns : list (fin 2)) :
@@ -89,74 +106,75 @@ Section BernoulliImpl.
     ⊢  WP e [{ Φ }]
   .
   Proof.
-    iIntros (HNone) "[(%l & Hα & %Htl) Hnext]".
+    iIntros (H_e_not_val) "[(%l & Hα & %Htl) Hnext]".
     wp_apply twp_presample; first done.
     iFrame.
     iIntros (k) "Htape".
-    destruct (decide (N ≤ k)) as [N_le_k | k_lt_N%not_le].
-    - iApply "Hnext".
-      iFrame.
-      iPureIntro.
-      by apply is_bernoulli_translation_app_0.
-    - iApply "Hnext".
-      iFrame.
-      iPureIntro.
-      by apply is_bernoulli_translation_app_1.
+    iApply ("Hnext" $! if (decide (N ≤ k)) then 0 else 1)%fin.
+    iFrame.
+    iPureIntro.
+    case_decide.
+    - apply is_bernoulli_translation_app_0 => //.
+    - apply is_bernoulli_translation_app_1 => //.
   Qed.
+
+  (**
+    Adaptation of the presample_adv_comp lemma for bernoulli distribution
+  *)
   Lemma twp_presample_bernoulli_adv_comp 
       (e : expr) (α : loc) (Φ : val → iProp Σ)
       (N M : nat) (ns : list (fin 2)) (ε : R)
       (D : fin 2 → R) :
     (N ≤ M + 1)%nat →
     (∀ (i : fin 2), 0 <= D i)%R →
-    (D 0%fin * (1 - (N / (M + 1))) + D 1%fin * (N / (M + 1)) = ε)%R
-    →  to_val e = None
-    → own_bernoulli_tape α N M ns ∗ ↯ ε ∗
+    D 0%fin * (1 - (N / (M + 1))) + D 1%fin * (N / (M + 1)) = ε →
+    to_val e = None →
+    ↯ ε ∗
+    own_bernoulli_tape α N M ns ∗ 
     (∀ (i : fin 2), ↯ (D i) ∗ own_bernoulli_tape α N M (ns ++ [i]) -∗ WP e [{ Φ }])
     ⊢  WP e [{ Φ }]
   .
   Proof.
-    iIntros (N_le_SM D_nonneg D_expected_ε HNone) "((%l & Hα & %Htl) & Herr & Hnext)".
+    iIntros (H_N_le_SM H_D_nonneg H_D_expected_ε H_e_not_val) "(Herr & (%l & Hα & %Htl) & Hnext)".
     set f :=
       λ (n : fin (S M)), 
         if bool_decide (fin_to_nat n < N)%nat then D 1%fin else D 0%fin.
     wp_apply (twp_presample_adv_comp _ M _ _ _ _ _ _ f); unfold f; first done; last iFrame.
-    { move=>>.
-      case_bool_decide; apply D_nonneg.
-    }
+    { move=>>. case_bool_decide; apply H_D_nonneg. }
     { rewrite SeriesC_scal_l. rewrite Rmult_comm.
       simpl_expr.
       Opaque INR.
       rewrite SeriesC_case //=.
-      rewrite -S_INR in D_expected_ε.
-      rewrite -D_expected_ε Rmult_plus_distr_l -!Rmult_assoc
+      rewrite -S_INR in H_D_expected_ε.
+      rewrite -H_D_expected_ε Rmult_plus_distr_l -!Rmult_assoc
                  !(Rmult_comm _ (D _)) !Rmult_assoc.
       simpl_expr.
       rewrite Rmult_minus_distr_l.
-      simpl_expr.
-    }
+      simpl_expr. }
     iIntros (n) "[Herr Hα]".
-    case_bool_decide;
-      wp_apply "Hnext";
-      iFrame;
-      iPureIntro.
+    wp_apply ("Hnext" $! if bool_decide (n < N)%nat then 1 else 0)%fin.
+    setoid_rewrite <-ssrbool.fun_if.
+    iFrame.
+    iPureIntro.
+    case_bool_decide.
     - apply is_bernoulli_translation_app_1 => //. 
     - apply is_bernoulli_translation_app_0 => //.
   Qed.
     
 
+  (**
+    Specification of the bernoulli function with tapes
+  *)
   Lemma twp_bernoulli_tape (N M : nat) (α : loc) (ns : list (fin 2)) (n : fin 2) :
     [[{ own_bernoulli_tape α N M (n::ns) }]]
       bernoulli (#lbl:α) #N #M
     [[{ RET #n ; own_bernoulli_tape α N M ns }]].
   Proof.
-    iIntros (Φ) "Htape HΦ".
-    rewrite /bernoulli {1}/own_bernoulli_tape.
-    iDestruct "Htape" as "(%l & Hα & %Htl)".
+    iIntros (Φ) "(%l & Hα & %Htl) HΦ".
+    rewrite /bernoulli.
     case: l Htl => [Hcontra | h t Htl]; first by apply is_bernoulli_translation_length in Hcontra. 
     wp_pures.
-    wp_apply (twp_rand_tape with "Hα").
-    iIntros "Hα".
+    wp_apply (twp_rand_tape with "Hα") as "Hα".
     wp_pures.
     apply is_bernoulli_translation_cons in Htl as [(-> & HNleh & Htl)| (-> & HhltN & Htl)]; bool_decide.
     - wp_pures.
@@ -167,7 +185,9 @@ Section BernoulliImpl.
       by iFrame.
   Qed.
 
-
+  (**
+    Adaptation of the planner lemma for the bernoulli distribution
+  *)
   Lemma twp_presample_bernoulli_planner 
       (N M : nat) (e : expr) (ε : nonnegreal)
       (L : nat) (α : loc) (Φ : val → iProp Σ)
@@ -177,32 +197,28 @@ Section BernoulliImpl.
     (∀ junk : list (fin 2),
        (0 < length (suffix (prefix ++ junk)) <= L)%nat) →
     0 < ε →
-    ↯ ε ∗ own_bernoulli_tape α N M prefix ∗
-    ( (∃ (junk : list (fin 2)), own_bernoulli_tape α N M (prefix ++ junk ++ suffix (prefix ++ junk))) -∗ WP e [{ Φ }]
+    ↯ ε ∗ 
+    own_bernoulli_tape α N M prefix ∗
+    ((∃ (junk : list (fin 2)), own_bernoulli_tape α N M (prefix ++ junk ++ suffix (prefix ++ junk))) -∗ WP e [{ Φ }]
     ) ⊢ WP e [{ Φ }].
   Proof.
-    iIntros ([zero_lt_N N_lt_SM] e_not_val suff_bound ε_pos)
+    iIntros ([H_zero_lt_N H_N_lt_SM] H_e_not_val H_suff_bound H_ε_pos)
       "(Herr & (%l & Hα & %Htl) & Hnext)".
     set suffix2 := bernoulli_to_tape M ∘ suffix ∘ tape_to_bernoulli N M.
-    wp_apply (twp_presample_planner_pos _ M _ _ _ _ _ L l suffix2); try done.
-    {
-      move=>>.
-      rewrite /suffix2 bernoulli_to_tape_length tape_to_bernoulli_app.
-      by apply tape_to_bernoulli_translation in Htl as <-.
-    }
-    iFrame.
-    iIntros "(%junk & Hα)".
+    wp_apply (twp_presample_planner_pos _ M _ _ _ _ _ L l suffix2 with "[$Herr $Hα Hnext]") as "(%junk & Hα)"; try done.
+    { move=>>. rewrite /suffix2 bernoulli_to_tape_length tape_to_bernoulli_app.
+      by apply tape_to_bernoulli_translation in Htl as <-. }
     iApply "Hnext".
-    iExists (tape_to_bernoulli N M junk), _.
     iFrame.
+    iExists (tape_to_bernoulli N M junk).
     iPureIntro.
     apply tape_to_bernoulli_translation.
-    rewrite !tape_to_bernoulli_app.
     apply tape_to_bernoulli_translation in Htl as ->.
-    rewrite -tape_to_bernoulli_app /suffix2 bernoulli_to_tape_to_bernoulli //=.
+    rewrite !tape_to_bernoulli_app -tape_to_bernoulli_app /suffix2 bernoulli_to_tape_to_bernoulli //=.
   Qed.
+  
 
   #[global] Instance bernoulli_impl : bernoulli_spec bernoulli :=
-    BernoulliSpec _ _ _ twp_bernoulli_scale bernoulli_case own_bernoulli_tape twp_presample_bernoulli twp_presample_bernoulli_adv_comp twp_bernoulli_tape twp_presample_bernoulli_planner.
+    BernoulliSpec _ _ bernoulli twp_bernoulli_scale bernoulli_case own_bernoulli_tape twp_presample_bernoulli twp_presample_bernoulli_adv_comp twp_bernoulli_tape twp_presample_bernoulli_planner.
   
 End BernoulliImpl.
