theories/eris/lib/sampling/bernoulli/interface.v
@@ -5,77 +5,69 @@ From clutch.eris.lib.sampling Require Import utils.
 
 Class bernoulli_spec `{!erisGS Σ} (bernoulli_prog : val) :=
   BernoulliSpec {
-      
-      twp_bernoulli_scale :
-      ∀ (N M : nat) (ε ε1 ε2 : R) 
-        (p := N / S M),
-        N ≤ S M →
-        0 <= ε1 →
-        0 <= ε2 →
-        ε1 * (1 - p) + ε2 * p = ε →
-        [[{↯ ε}]]
-          bernoulli_prog #() #N #M
-          [[{
-                (k : nat), RET #k;
-                (⌜k = 0%nat⌝ ∗ ↯ ε1) ∨
-                  (⌜k = 1%nat⌝ ∗ ↯ ε2)
-          }]];
-
-  bernoulli_case :
-      ∀ (N M : nat),
-        (*TODO: See to add N <= S M  *)
-        [[{True}]]
-          bernoulli_prog #() #N #M
-          [[{v, RET v; ⌜v = #0⌝ ∨ ⌜v = #1⌝}]];
+    twp_bernoulli_scale (N M : nat) (ε ε1 ε2 : R) (p := N / S M) :
+      N ≤ S M →
+      0 <= ε1 →
+      0 <= ε2 →
+      ε1 * (1 - p) + ε2 * p = ε →
+      [[{↯ ε}]]
+        bernoulli_prog #() #N #M
+      [[{
+        (k : nat), RET #k;
+        (⌜k = 0%nat⌝ ∗ ↯ ε1) ∨
+        (⌜k = 1%nat⌝ ∗ ↯ ε2)
+      }]];
 
   own_bernoulli_tape :
       loc → nat → nat → list (fin 2) → iPropI Σ;
-  
-  twp_presample_bernoulli : 
-      ∀ (e : expr) (α : loc) (Φ : val → iProp Σ) 
-        (N M : nat) (ns : list (fin 2)),
-        to_val e = None →
-        own_bernoulli_tape α N M ns ∗ 
-        (∀ i : fin 2, 
-           own_bernoulli_tape α N M (ns ++ [i]) -∗ WP e [{ v, Φ v }]) 
-        ⊢ WP e [{ v, Φ v }];
-  
-  twp_presample_bernoulli_adv_comp : 
-      ∀ (e : expr) (α : loc) (Φ : val → iProp Σ) 
-        (N M : nat) (ns : list (fin 2)) (ε : R) (D : fin 2 → R),
-        N ≤ M + 1 →
-        (∀ i : fin 2, 0 <= D i) →
-        D 0%fin * (1 - N / (M + 1)) + D 1%fin * (N / (M + 1)) = ε →
-        to_val e = None → 
-        own_bernoulli_tape α N M ns ∗ 
-        ↯ ε ∗ 
-        (∀ i : fin 2, 
-           ↯ (D i) ∗ own_bernoulli_tape α N M (ns ++ [i]) -∗ 
-           WP e [{ v, Φ v }])
-        ⊢ WP e [{ v, Φ v }];
 
-  twp_bernoulli_tape :
-      ∀ (N M : nat) (α : loc) (ns : list (fin 2)) (n : fin 2),
-        [[{ own_bernoulli_tape α N M (n::ns) }]]
-          bernoulli_prog (#lbl:α) #N #M
-          [[{ RET #n ; own_bernoulli_tape α N M ns }]];
-      
-      twp_presample_bernoulli_planner :
-      ∀ (N M : nat) (e : expr) (ε : nonnegreal) (L : nat) 
-        (α : loc) (Φ : val → iProp Σ) (prefix : list (fin 2)) 
-        (suffix : list (fin 2) → list (fin 2)),
-        (0 < N < S M)%nat →
-        to_val e = None →
-        (∀ junk : list (fin 2), 
-           (0 < length (suffix (prefix ++ junk)) <= L)%nat) → 
-        0 < ε → 
-        ↯ ε ∗ 
-        own_bernoulli_tape α N M prefix ∗
-        ((∃ junk : list (fin 2), 
-      own_bernoulli_tape α N M (prefix ++ junk ++ suffix (prefix ++ junk))) 
-         -∗ WP e [{ v, Φ v }])
-        ⊢ WP e [{ v, Φ v }]
-    }.
+
+  twp_presample_bernoulli 
+      (e : expr) (α : loc) (Φ : val → iProp Σ) 
+      (N M : nat) (ns : list (fin 2)) : 
+    to_val e = None →
+    own_bernoulli_tape α N M ns ∗ 
+    (∀ i : fin 2, own_bernoulli_tape α N M (ns ++ [i]) -∗ WP e [{ v, Φ v }]) 
+    ⊢ WP e [{ v, Φ v }];
+
+
+  twp_presample_bernoulli_adv_comp 
+      (e : expr) (α : loc) (Φ : val → iProp Σ) 
+      (N M : nat) (ns : list (fin 2)) (ε : R) (D : fin 2 → R): 
+    N ≤ M + 1 →
+    (∀ i : fin 2, 0 <= D i) →
+    D 0%fin * (1 - N / (M + 1)) + D 1%fin * (N / (M + 1)) = ε →
+    to_val e = None → 
+    ↯ ε ∗ 
+    own_bernoulli_tape α N M ns ∗ 
+    (∀ i : fin 2, 
+        ↯ (D i) ∗ own_bernoulli_tape α N M (ns ++ [i]) -∗ 
+        WP e [{ v, Φ v }])
+    ⊢ WP e [{ v, Φ v }];
+
+
+  twp_bernoulli_tape (N M : nat) (α : loc) (ns : list (fin 2)) (n : fin 2) :
+    [[{ own_bernoulli_tape α N M (n::ns) }]]
+      bernoulli_prog (#lbl:α) #N #M
+    [[{ RET #n ; own_bernoulli_tape α N M ns }]];
+
+
+  twp_presample_bernoulli_planner 
+      (N M : nat) (e : expr) (ε : nonnegreal) (L : nat) 
+      (α : loc) (Φ : val → iProp Σ) (prefix : list (fin 2)) 
+      (suffix : list (fin 2) → list (fin 2)) :
+    (0 < N < S M)%nat →
+    to_val e = None →
+    (∀ junk : list (fin 2), 
+        (0 < length (suffix (prefix ++ junk)) <= L)%nat) → 
+    0 < ε → 
+    ↯ ε ∗ 
+    own_bernoulli_tape α N M prefix ∗
+    ((∃ junk : list (fin 2), 
+        own_bernoulli_tape α N M (prefix ++ junk ++ suffix (prefix ++ junk))) -∗ 
+      WP e [{ v, Φ v }])
+    ⊢ WP e [{ v, Φ v }]
+}.
 
 Set Default Proof Using "Type*".
 
@@ -92,8 +84,19 @@ Section BernoulliSpecLemmas.
       real_solver  |
       tactics.done |
       auto
-      ].
-  
+    ].
+  Lemma bernoulli_case (N M : nat) :
+    N ≤ S M →
+    [[{True}]]
+      bernoulli #() #N #M
+    [[{v, RET v; ⌜v = #0⌝ ∨ ⌜v = #1⌝}]].
+  Proof.
+    iIntros "% %Φ _ HΦ".
+    iMod ec_zero as "Herr".
+    wp_apply (twp_bernoulli_scale N M _ 0 0 with "Herr")%R as "% [[-> _] | [-> _]]" => //;
+    iApply "HΦ" => //.
+  Qed.
+
   Lemma bernoulli_success_spec (N M : nat) (ε ε' : R) (p := N / S M) :
     (0 <= ε')%R →
     ε = (ε' * (N / S M)) → 
@@ -102,10 +105,11 @@ Section BernoulliSpecLemmas.
     [[{ v, RET v; ↯ ε' ∗ ⌜v = #1⌝ }]].
   Proof.
     iIntros (Hε' ->) "%Φ [Herr Hcost] HΦ".
-    destruct (decide (S M < N)%nat) as [Hlt | Hge%not_lt].
-    { cred_contra. rewrite Rcomplements.Rlt_minus_l. simpl_expr. }
+    iAssert (⌜N ≤ S M⌝)%I with "[Hcost]" as "%H_N_le_SM".
+    { destruct (decide (S M < N)%nat); last by iPureIntro; done.
+      cred_contra. rewrite Rcomplements.Rlt_minus_l. simpl_expr. }
     iPoseProof (ec_combine with "[$Herr $Hcost]") as "Herr".
-    wp_apply (twp_bernoulli_scale _ _ _ 1 ε' with "Herr")%R; [lia|lra..|].
+    wp_apply (twp_bernoulli_scale _ _ _ 1 ε' with "Herr")%R; try done.
     iIntros "%k [(_ & Herr) | (-> & Herr)]"; first cred_contra. 
     by iApply "HΦ"; iFrame.
   Qed.
@@ -117,7 +121,7 @@ Section BernoulliSpecLemmas.
   Proof.
     iIntros (Φ) "Herr HΦ".
     iMod ec_zero as "Hzero".
-    wp_apply (bernoulli_success_spec _ _ 0%R 0%R with "[$Herr $Hzero]") as "%v [_ Hv]" => //.
+    wp_apply (bernoulli_success_spec _ _ 0 0 with "[$Herr $Hzero]") as "%v [_ Hv]" => //.
     iApply ("HΦ" with "Hv").
   Qed.
 
@@ -129,11 +133,12 @@ Section BernoulliSpecLemmas.
     [[{ v, RET v; ↯ ε' ∗ ⌜v = #0⌝ }]].
   Proof.
     iIntros (Hε ->) "%Φ [Herr Hcost] HΦ".
-    destruct (decide (S M < N)%nat) as [Hlt |Hge%not_lt].
-    { cred_contra. simpl_expr. }
+    iAssert (⌜N ≤ S M⌝)%I with "[Hcost]" as "%H_N_le_SM".
+    { destruct (decide (S M < N)%nat) as [Hlt |Hge%not_lt];
+      [cred_contra; simpl_expr | done]. }
     iPoseProof (ec_combine with "[$Herr $Hcost]") as "Herr".
     wp_apply (twp_bernoulli_scale _ _ _ ε' 1 with "[$Herr]")%R => //.
-    iIntros "%k [(-> & Herr) | (-> & Herr)]";last cred_contra.
+    iIntros "%k [(-> & Herr) | (-> & Herr)]"; last cred_contra.
     by iApply "HΦ"; iFrame.
   Qed.
 
